\begin{problem}{1.1}
    Apply Notation 1.3.10 on the follwoing $\lambda$-terms. SO, remove parentheses and combine $lambda$-abstractions:
    \begin{enumerate}
        \item $(\lambda x.(((xz)y)(xx)))$
        \item $((\lambda x.(\lambda y.(\lambda z .(z((xy)z)))))(\lambda u.u))$
    \end{enumerate}
\end{problem}

\begin{solution}
    \begin{enumerate}
        \item $(\lambda x.(((xz)y)(xx)))$ = $\lambda x. ((xz)y)(xx)$ = $\lambda x. (xz)y(xx)$ = $\lambda x. (xz)y(xx)$ = $\lambda x. xzy(xx)$
        \item Final answer: $\lambda xyz. z((xy)z)(\lambda u.u)$
    \end{enumerate}
\end{solution}