\begin{problem}{1.12}
    We define the \(\lambda\)-terms \(\mathit{true}\) and \(\mathit{false}\) (the \emph{booleans}) and \(\mathit{not}\) (resembling the logical \(\neg\)-operator) by:
    $$ \mathit{true} := \lambda xy\,.\, x \quad \text{(so it happens that } \mathit{true} \equiv \mathsf{K}), $$
    $$ \mathit{false} := \lambda xy\,.\, y \quad \text{(and } \mathit{false} \equiv \mathit{zero}). $$
    $$ \mathit{not} := \lambda z.z \;\; false \;\; true $$
    Show that $not \;\; not \;\; p =_\beta p$ for all terms $p$, in each of the two cases:
    \begin{enumerate}[label=$(\alph*)$]
        \item $p \twoheadrightarrow_\beta true$
        \item $p \twoheadrightarrow_\beta false$
    \end{enumerate}
\end{problem}

\begin{solution}
    It is sufficient to show that $not \;\; true \twoheadrightarrow_\beta false$ and $not \;\; false \twoheadrightarrow_\beta true$.
    $$ not \;\; true = (\lambda z.z (\lambda ab.b) (\lambda ab.a)) (\lambda ab.a) \to_\beta (\lambda ab.a)(\lambda ab.b)(\lambda ab.a) \to_\beta \lambda ab.b = false $$
    similarly, $not \;\; false \twoheadrightarrow_\beta true$.
\end{solution}