\begin{problem}{1.2}
    Find out for each of the following $\lambda$-terms whether it is $\alpha$-equivalent, or not, to $\lambda x.x(\lambda x.x)$:
    \begin{enumerate}[label=$(\alph*)$]
        \item $\lambda y.y(\lambda x.x)$
        \item $\lambda y.y(\lambda x.y)$
        \item $\lambda y.y(\lambda y.x)$
    \end{enumerate}
\end{problem}

\begin{solution}
    The original term is $\lambda x.x (\lambda x.x) =_\alpha \lambda a.a (\lambda b.b)$.
    With this clarification on the original term, it is obvious that it is $\alpha$-equivalent to only the first term.
\end{solution}