\begin{problem}{1.4}
    Consider the following $\lambda$-term: 
    $$ U := \underbrace{(\lambda z.zxz)}_{A} \underbrace{((\lambda y.xy)x)}_{B} $$
    \begin{enumerate}[label=$(\alph*)$]
        \item Give a list of all subterms of $U$
        \item Draw the tree representation of $U$
        \item Find the set of all free variables of $U$ by a calculation, as in Examples 1.4.2.
        \item Find out which of the following $\lambda$-terms are $\alpha$-equivalent to $U$ and give motivation why; also check which of them satisfies the Barendregt convention
            \begin{enumerate}[label=$\roman*.$]
                \item $(\lambda y.yxy)((\lambda z.xz)x)$,
                \item $(\lambda x.xyx)((\lambda z.yz)y)$,
                \item $(\lambda y.yxy)((\lambda y.xy)x)$,
                \item $(\lambda v.(vx)v)((\lambda u.uv)x)$.
            \end{enumerate}
    \end{enumerate}
\end{problem}

\begin{solution}
    \begin{enumerate}[label=$(\alph*)$]
        \item $sub(U) = sub(A) \cup sub(B)$ where \\ $sub(A) = \{ \lambda z.zxz, zxz, z, x, z, zx \}$ 
            and \\ $sub(B) = \{ (\lambda y.xy)x, \lambda y.xy, x, x, y, xy  \}$
        
        \item Easy!
        \item $FV(U) = FV(A) \cup FV(B) = (FV(zxz) \backslash \{z\}) \cup ((FV(xy) \backslash \{y\}) \cup \{x\}) = \{ x \}$
        \item \begin{enumerate}[label=$\roman*.$]
            \item Obviously, this is $\alpha$-equivalent to the term $U$ and it satisfies the Barendregt convention.
            \item The free variables $x$ in $B$ has changed to $y$. Hence, it is not equivalent to $U$. However, it satisfies the Barendregt convention.
            \item Yes, they are are equivalent since only the bound variable $z$ is change to $y$ in $A$. However, it does not satisfy the Barendregt convention for obvious reasons.
            \item The free variable $x$ in $B$ has changed to $v$, making them not to be equivalent. It also does not satisfy the Barendregt convention since $v$ occurs as both bound and free variable.  
        \end{enumerate}
    \end{enumerate}
\end{solution}