\begin{problem}{1.5}
    Give the results of the following substitutions:
    \begin{enumerate}[label=$(\alph*)$]
        \item $(\lambda x \cdot y (\lambda y \cdot x \, y)) [y := \lambda z \cdot z \, x]$, 
        \item $((x \, y \, z) [x := y]) [y := z]$, 
        \item $((\lambda x \cdot x \, y \, z) [x := y]) [y := z]$, 
        \item $(\lambda y \cdot y \, y \, x) [x := y \, z]$.
    \end{enumerate}
\end{problem}

\begin{solution}
    \begin{enumerate}[label=$(\alph*)$]
        \item First of all, $\lambda x.y(\lambda y.xy) =_\alpha \lambda a.y(\lambda b.ab)$. Hence, the result of the substitution would be $(\lambda a.(\lambda z.zx)(\lambda b.ab))$.
        \item $ ((xyz)[x := y])[y:=z] = (yyz)[y:=z] = (zzz) $
        \item $ (\lambda x.xyz) =_\alpha (\lambda a.ayz) $, and the substitution would be: $$ ((\lambda a.ayz)[x:=y])[y:=z] = (\lambda a.ayz)[y:=z] = (\lambda a.azz) $$
        \item $ (\lambda y.yyx) =_\alpha (\lambda a.aax) \Rightarrow (\lambda a.aax)[x:=yz] = (\lambda a.aayz) $
    \end{enumerate}
\end{solution}