\begin{problem}{3.14}
    We may also introduce the polymorphic booleans in $\lambda 2$:
    $$\mathit{Bool} \equiv \Pi\alpha:* \cdot \alpha\rightarrow\alpha\rightarrow\alpha,$$
    $$\mathit{True} \equiv \lambda\alpha:* \cdot \lambda x,y:\alpha \cdot x,$$
    $$\mathit{False} \equiv \lambda\alpha:* \cdot \lambda x,y:\alpha \cdot y.$$
    Construct a $\lambda 2$-term $\mathit{Neg}:\mathit{Bool}\to \mathit{Bool}$ such that $\mathit{Neg}\ \mathit{True}=_\beta \mathit{False}$ and $\mathit{Neg}\ \mathit{False}=_\beta \mathit{True}$. Prove the correctness of your answer.
\end{problem}

\begin{solution}
    Define: $$ Neg \equiv \lambda b : Bool . \lambda \alpha : * . \lambda x, y : \alpha . b\ \alpha\ y\ x : Bool \to Bool $$

We show that $Neg : Bool \rightarrow Bool$ and that it satisfies the required properties.
    $$Neg \; True =_\beta False$$
\begin{align*}
Neg\ True 
&= (\lambda b : Bool . \lambda \alpha : * . \lambda x : \alpha . \lambda y : \alpha . b\ \alpha\ y\ x)\ True \\[6pt]
&\;\;\;\;\;\rightarrow_\beta \lambda \alpha : * . \lambda x : \alpha . \lambda y : \alpha . True\ \alpha\ y\ x \\[6pt]
&= \lambda \alpha : * . \lambda x : \alpha . \lambda y : \alpha . (\lambda \alpha : * . \lambda x : \alpha . \lambda y : \alpha . x)\ \alpha\ y\ x \\[6pt]
&\;\;\;\;\;\rightarrow_\beta \lambda \alpha : * . \lambda x : \alpha . \lambda y : \alpha . (\lambda x : \alpha . \lambda y : \alpha . x)\ y\ x \\[6pt]
&\;\;\;\;\;\rightarrow_\beta \lambda \alpha : * . \lambda x : \alpha . \lambda y : \alpha . (\lambda y : \alpha . y)\ x \\[6pt]
&\;\;\;\;\;\rightarrow_\beta \lambda \alpha : * . \lambda x : \alpha . \lambda y : \alpha . y \\[6pt]
&= False
\end{align*}

Similarly, it can be shown that $Neg \; False =_\beta True$.
\end{solution}